src/RqDownRed.v
@@ -19,5 +19,55 @@ Section RqDownReduction.
 
   Hypothesis (Hrrs: RqRsSys dtr sys).
 
+  Section OnRqDown.
+    Variables (oidxTo: IdxT)
+              (rqDowns: list (Id Msg)).
+    Hypothesis (Hrqd: RqDownMsgs dtr oidxTo rqDowns).
+
+    Lemma rqDown_oinds:
+      forall inits ins hst outs eouts,
+        SubList rqDowns eouts ->
+        Atomic msg_dec inits ins hst outs eouts ->
+        forall st1 st2,
+          Reachable (steps step_m) sys st1 ->
+          steps step_m sys st1 hst st2 ->
+          DisjList (oindsOf hst) (subtreeIndsOf dtr oidxTo).
+    Proof.
+    Admitted.
+
+    Lemma rqDown_olast_inside_tree:
+      forall inits ins hst outs eouts,
+        DisjList inits rqDowns ->
+        Atomic msg_dec inits ins hst outs eouts ->
+        forall st1 st2 loidx,
+          Reachable (steps step_m) sys st1 ->
+          Forall (InMPI st1.(bst_msgs)) rqDowns ->
+          steps step_m sys st1 hst st2 ->
+          lastOIdxOf hst = Some loidx ->
+          In loidx (subtreeIndsOf dtr oidxTo) ->
+          SubList (oindsOf hst) (subtreeIndsOf dtr oidxTo).
+    Proof.
+    Admitted.
+
+    Lemma rqDown_olast_outside_tree:
+      forall inits ins hst outs eouts,
+        DisjList inits rqDowns ->
+        Atomic msg_dec inits ins hst outs eouts ->
+        forall st1 st2 loidx,
+          Reachable (steps step_m) sys st1 ->
+          Forall (InMPI st1.(bst_msgs)) rqDowns ->
+          steps step_m sys st1 hst st2 ->
+          lastOIdxOf hst = Some loidx ->
+          ~ In loidx (subtreeIndsOf dtr oidxTo) ->
+          exists rqUps phst nhst,
+            hst = nhst ++ phst /\
+            RqUpHistory dtr phst rqUps /\
+            SubList (oindsOf phst) (subtreeIndsOf dtr oidxTo) /\
+            DisjList (oindsOf nhst) (subtreeIndsOf dtr oidxTo).
+    Proof.
+    Admitted.
+
+  End OnRqDown.
+
 End RqDownReduction.
 
