src/RsUpRed.v
@@ -182,19 +182,6 @@ Section RsUpReduction.
     try disc_msgs_in;
     try disc_rqToUpRule.
 
-  Ltac solve_midx_disj :=
-    repeat
-      match goal with
-      | [ |- _ <> _] => solve_midx_neq
-      | [ |- ~ In _ _] => solve_midx_neq
-      | [ |- DisjList (_ :: nil) (_ :: nil)] =>
-        apply (DisjList_singletons eq_nat_dec)
-      | [ |- DisjList (_ :: nil) _] =>
-        apply (DisjList_singleton_1 eq_nat_dec)
-      | [ |- DisjList _ (_ :: nil)] =>
-        apply (DisjList_singleton_2 eq_nat_dec)
-      end.
-
   Lemma rsUp_lbl_reducible:
     forall oidxTo rsUps,
       RsUpMsgs dtr oidxTo rsUps ->
